x86model/RockSalt/VerifierDFA.v
@@ -31,7 +31,7 @@ Require ExtrOcamlString.
 Require ExtrOcamlNatBigInt.
 Require ExtrOcamlNatInt.
 Import ParserArg.X86_PARSER_ARG.
-Import X86_PARSER.
+(* Import X86_PARSER. *)
 (* Import X86_BASE_PARSER. *)
 Require Import X86Syntax.
 
